src/LocalsOnlyComp.v
@@ -53,6 +53,15 @@ Definition compile_list_list :=
         | e :: es => go_list e :: go_list_list es
         end in go_list_list.
 
+Definition compile_func (f : list A.insn * nat) : list B.insn * nat :=
+    let '(body, ret) := f in
+    (compile_list body, ret).
+
+Definition compile_cu (cu : list (list A.insn * nat) * list metadata) :
+        list (list B.insn * nat) * list metadata :=
+    let '(funcs, metas) := cu in
+    (map compile_func funcs, metas).
+
 Ltac refold_compile :=
     fold compile_list in *;
     fold compile_list_list in *.
@@ -113,7 +122,7 @@ Inductive I : A.state -> B.state -> Prop :=
 
 
 
-Theorem compile_I_expr : forall a b,
+Lemma compile_I_insn : forall a b,
     compile a = b ->
     I_insn a b.
 induction a using A.insn_rect_mut with
@@ -126,6 +135,32 @@ induction a using A.insn_rect_mut with
 intros0 Hcomp; simpl in Hcomp; try rewrite <- Hcomp; refold_compile;
 try solve [econstructor; eauto].
 Qed.
+
+Lemma compile_list_I_insn : forall a b,
+    compile_list a = b ->
+    Forall2 I_insn a b.
+induction a;
+intros0 Hcomp; simpl in Hcomp; try rewrite <- Hcomp; refold_compile;
+try solve [econstructor; eauto using compile_I_insn].
+Qed.
+
+Lemma compile_I_func : forall a b,
+    compile_func a = b ->
+    I_func a b.
+intros0 Hcomp.
+unfold compile_func in Hcomp. break_match. rewrite <- Hcomp.
+constructor; eauto using compile_list_I_insn.
+Qed.
+
+Theorem compile_cu_I_env : forall a ameta b bmeta,
+    compile_cu (a, ameta) = (b, bmeta) ->
+    Forall2 I_func a b.
+intros0 Hcomp. unfold compile_cu in *. inject_pair.
+remember (map compile_func a) as b.
+symmetry in Heqb. apply map_Forall2 in Heqb.
+list_magic_on (a, (b, tt)). eauto using compile_I_func.
+Qed.
+
 
 
 
