src/LocalsCompCombined.v
@@ -1,0 +1,102 @@
+Require Import compcert.driver.Compiler compcert.common.Errors.
+Require Import Common Monads.
+Require CompilationUnit.
+Require Import Metadata.
+
+Require StackFlatter2 LocalsOnlyComp.
+Require
+    LocalsDestsComp
+    LocalsSwitchComp
+    LocalsReturnComp
+    LocalsSourcesComp
+    LocalsOnlyComp
+.
+
+Definition option_to_res {A} (o : option A) : res A :=
+  match o with
+  | None => Error []
+  | Some a => OK a
+  end.
+Coercion option_to_res : option >-> res.
+
+Definition compile_cu (cu : StackFlatter2.env * list metadata) :
+        res (LocalsOnly.env * list metadata) :=
+  OK cu
+  @@ LocalsDestsComp.compile_cu
+  @@ LocalsSwitchComp.compile_cu
+  @@ LocalsReturnComp.compile_cu
+ @@@ LocalsSourcesComp.compile_cu
+  @@ LocalsOnlyComp.compile_cu
+.
+
+Inductive I : StackFlatter2.state -> LocalsOnly.state -> Prop :=
+| ICombined : forall s00 s01 s02 s03 s04 s05,
+        LocalsDestsComp.I   s00 s01 ->
+        LocalsSwitchComp.I  s01 s02 ->
+        LocalsReturnComp.I  s02 s03 ->
+        LocalsSourcesComp.I s03 s04 ->
+        LocalsOnlyComp.I    s04 s05 ->
+        I s00 s05.
+
+Inductive I_func : list StackFlatter2.insn -> list LocalsOnly.insn * nat -> Prop :=
+| IFuncCombined : forall f00 f01 f02 f03 f04 f05,
+        Forall2 LocalsDestsComp.I_insn      f00 f01 ->
+        Forall2 LocalsSwitchComp.I_insn     f01 f02 ->
+        LocalsReturnComp.I_func             f02 f03 ->
+        LocalsSourcesComp.I_func            f03 f04 ->
+        LocalsOnlyComp.I_func               f04 f05 ->
+        I_func f00 f05.
+
+
+Lemma chain_I_env :
+    forall e00 e01 e02 e03 e04 e05,
+        Forall2 (Forall2 LocalsDestsComp.I_insn)    e00 e01 ->
+        Forall2 (Forall2 LocalsSwitchComp.I_insn)   e01 e02 ->
+        Forall2 (LocalsReturnComp.I_func)           e02 e03 ->
+        Forall2 (LocalsSourcesComp.I_func)          e03 e04 ->
+        Forall2 (LocalsOnlyComp.I_func)             e04 e05 ->
+        Forall2 I_func e00 e05.
+intros.
+list_magic_on (e00, (e01, (e02, (e03, (e04, (e05, tt)))))).
+eapply IFuncCombined; eassumption.
+Qed.
+
+
+Ltac break_result_chain :=
+    let go l :=
+        match l with
+        | OK _ => fail 1
+        | _ => destruct l eqn:?; try discriminate
+        end in
+    repeat match goal with
+    | [ H : context [ ?l @@ ?r ] |- _ ] => go l
+    | [ H : context [ ?l @@@ ?r ] |- _ ] => go l
+    end.
+
+Ltac inject_ok :=
+    repeat match goal with
+    | [ H : OK ?x = OK ?y |- _ ] =>
+            assert (x = y) by congruence;
+            clear H
+    end.
+
+
+Theorem compile_I_func : forall a ameta b bmeta,
+    compile_cu (a, ameta) = OK (b, bmeta) ->
+    Forall2 I_func a b.
+intros0 Hcomp. unfold compile_cu in *.
+
+remember (a, ameta) as aprog.
+break_result_chain.  simpl in *.  inject_ok.
+unfold option_to_res in *. repeat (break_match; try discriminate).
+subst aprog.  repeat on (_ * _)%type, fun x => destruct x.
+
+on _, eapply_lem LocalsDestsComp.compile_cu_I_env.
+on _, eapply_lem LocalsSwitchComp.compile_cu_I_env.
+on _, eapply_lem LocalsReturnComp.compile_cu_I_env.
+on _, eapply_lem LocalsSourcesComp.compile_cu_I_env.
+on _, eapply_lem LocalsOnlyComp.compile_cu_I_env.
+
+inject_ok. inject_pair.
+eapply chain_I_env; eassumption.
+Qed.
